simplefmi/SimpleTank.thy
@@ -33,14 +33,14 @@ alphabet wt_st =
   ctr   :: "ctr_st vrt_st_scheme"
     
 definition
-  "Init = [ tank:valve      \<mapsto>\<^sub>s true
-          , tank:level      \<mapsto>\<^sub>s 0
-          , ctr:valveOn     \<mapsto>\<^sub>s false
-          , ctr:levelSensor \<mapsto>\<^sub>s 0 ]"
+  "Init = [ &tank:valve      \<mapsto>\<^sub>s true
+          , &tank:level      \<mapsto>\<^sub>s -0.001
+          , &ctr:valveOn     \<mapsto>\<^sub>s true
+          , &ctr:levelSensor \<mapsto>\<^sub>s 0 ]"
   
 definition 
-  "Wiring = [ tank:valve      \<mapsto>\<^sub>s &ctr:valveOn
-            , ctr:levelSensor \<mapsto>\<^sub>s &tank:level ]"
+  "Wiring = [ &tank:valve      \<mapsto>\<^sub>s &ctr:valveOn
+            , &ctr:levelSensor \<mapsto>\<^sub>s &tank:level ]"
 
 abbreviation (input) tank_ode_1 :: "real \<Rightarrow> real \<Rightarrow> real" where
 "tank_ode_1 \<equiv> (\<lambda> t l. 1)"
@@ -62,29 +62,76 @@ lemma tank_ode_usol_2:
   "l > 0 \<Longrightarrow> (tank_sol_2 l\<^sub>0 usolves_ode tank_ode_2 from 0) {0..l} UNIV"
   by (linear_ode)
     
-definition Tank  :: "real \<Rightarrow> tank_st fmu" where 
-  "Tank area = 
-    Modelica_FMU 
-      ((\<langle>{&level} : tank_ode_1(ti)\<rangle>\<^sub>h \<and> level \<leftarrow>\<^sub>h $level) 
-         \<triangleleft> &valve \<triangleright>\<^sub>h 
-       (\<langle>{&level} : tank_ode_2(ti)\<rangle>\<^sub>h \<and> level \<leftarrow>\<^sub>h $level))"
+definition Tank  :: "tank_st fmu" where 
+  "Tank = Modelica_FMU (\<langle>&level : \<lambda>lev. -1\<rangle>\<^sub>h \<triangleleft> &valve \<triangleright>\<^sub>h \<langle>&level : \<lambda>lev. 1\<rangle>\<^sub>h)"
 
 definition Ctr :: "real \<Rightarrow> real \<Rightarrow> ctr_st vrt_st_ext fmu" where
 "Ctr minLevel maxLevel = 
-  VDMRT_FMU 0.001 (valveOn := true \<triangleleft> &levelSensor \<le>\<^sub>u \<guillemotleft>minLevel + 0.2\<guillemotright> \<triangleright>\<^sub>r 
-                   valveOn := false \<triangleleft> &levelSensor \<ge>\<^sub>u \<guillemotleft>maxLevel - 0.2\<guillemotright> \<triangleright>\<^sub>r II)"
-
-lemma rel_frext_skip [alpha]: 
-  "vwb_lens a \<Longrightarrow> II \<oplus>\<^sub>f a = II"
-  by (rel_auto)
+  VDMRT_FMU 0.001 (valveOn := false \<triangleleft> &levelSensor \<le>\<^sub>u \<guillemotleft>minLevel\<guillemotright> \<triangleright>\<^sub>r 
+                   valveOn := true \<triangleleft> &levelSensor \<ge>\<^sub>u \<guillemotleft>maxLevel\<guillemotright> \<triangleright>\<^sub>r II)"
 
 definition 
-  "WaterTank minLevel maxLevel area = 
-     FMI Init [FMU[ctr, Ctr minLevel maxLevel], FMU[tank, Tank area]] ArbStep Wiring"
-      
-lemma "FMI Init [FMU[ctr, Ctr minLevel maxLevel], FMU[tank, Tank area]] (FixedStep 1) Wiring = false"
-  apply (simp add: FMI_def Step_FMUs_def fmu_single_def Ctr_def VDMRT_FMU_def Modelica_FMU_def alpha usubst Tank_def)
+  "WaterTank minLevel maxLevel = 
+     FMI Init [FMU[ctr, Ctr minLevel maxLevel], FMU[tank, Tank]] ArbStep Wiring"
+   
+term "[x:y \<mapsto>\<^sub>s v]"
     
+
+(*
+term "\<sigma>(y ;\<^sub>L x \<mapsto>\<^sub>s v)"
+*)  
+
+translations 
+  "\<sigma>(x:y \<mapsto>\<^sub>s v)" <= "CONST subst_upd \<sigma> (y ;\<^sub>L x) v"
+
+term "assigns_r (subst_upd id (y ;\<^sub>L x) v)"
+  
+term "x:y := v" 
+                    
+declare [[show_types=false]]
+    
+text {* Use of a 1 second fixed step master algorithm when the VDM-RT model only permits 1ms or less
+  yields no possible evolutions, and thus only the initial state can be observed. *}
+    
+lemma st_subst_rel [usubst]:
+  "\<sigma> \<dagger>\<^sub>S [P]\<^sub>S = [\<lceil>\<sigma>\<rceil>\<^sub>s \<dagger> P]\<^sub>S"
+  by (rel_auto)
+      
+declare cond_st_distr [rpred del]
+    
+
+  
+  
+term "x := v"
+  
+term "(subst_upd id (y ;\<^sub>L x) v)"
+    
+term ctdown
+  
+lemma "ctr:ctdown :=\<^sub>r 0 ;; ctr:valveOn :=\<^sub>r false = undefined"
+  apply (simp add: rpred closure usubst)
+  oops
+    
+lemma ArbStep_not_empty [simp]: "\<not> ArbStep = {}"
+  by (simp add: ArbStep_def)
+
+lemma st_subst_comp [usubst]: 
+  "\<lceil>\<sigma>\<rceil>\<^sub>S\<^sub>\<sigma> \<circ> \<lceil>\<rho>\<rceil>\<^sub>S\<^sub>\<sigma> = \<lceil>\<sigma> \<circ> \<rho>\<rceil>\<^sub>S\<^sub>\<sigma>"
+  by (rel_auto)
+    
+lemma "FMI Init [FMU[ctr, Ctr 1 10], FMU[tank, Tank]] (FixedStep 1) Wiring = false"
+  apply (simp add: FMI_def alpha frame rpred usubst Ctr_def Tank_def FixedStep_def Init_def Step_FMUs_def seqr_assoc)
+  apply (subst rea_assigns_comp)
+    apply (simp_all add: closure)
+  apply (simp add: rpred closure usubst)
+  apply (subst rea_uplus_unfold)
+      apply (simp add: rpred closure usubst)
+   apply (simp add: rea_assigns_comp closure usubst frame unrest Step_VDMRT)
+  apply (literalise, simp, unliteralise)
+  apply (simp add: frame rpred alpha usubst unrest)
+  apply (uexpr_simp simps: pos_transfer, simp add: rpred)
+done
+  
   
 lemma tank_ode_1_evolve:
   "\<langle>{&level} : tank_ode_1(ti)\<rangle>\<^sub>h = {[&level \<mapsto>\<^sub>s \<guillemotleft>op +\<guillemotright>(&level)\<^sub>a(\<guillemotleft>ti\<guillemotright>)\<^sub>a]}\<^sub>h"
@@ -102,11 +149,265 @@ lemma continuous_lens_level [closure]: "continuous_lens level"
   apply (simp add: tank_st.select_defs iso_tuple_fst_def tuple_iso_tuple_def 
       tank_st_ext_Tuple_Iso_def Topological_Spaces.continuous_on_fst continuous_Rep_tank_st_ext)
   sorry
-    
-    
-lemma "H2T(\<langle>&level : \<lambda>lev. 1\<rangle>\<^sub>h \<triangleleft> &valve \<triangleright>\<^sub>h \<langle>&level : \<lambda>lev. - 1\<rangle>\<^sub>h) = 
+        
+lemma Tank_Step:
+  "H2T(\<langle>&level : \<lambda>lev. 1\<rangle>\<^sub>h \<triangleleft> &valve \<triangleright>\<^sub>h \<langle>&level : \<lambda>lev. - 1\<rangle>\<^sub>h) = 
        (\<Sqinter> t | 0 <\<^sub>u \<guillemotleft>t\<guillemotright> \<bullet> wait\<^sub>r \<guillemotleft>t\<guillemotright> ;; (level :=\<^sub>r (&level + \<guillemotleft>real_of_pos t\<guillemotright>) \<triangleleft> &valve \<triangleright>\<^sub>R level :=\<^sub>r (&level - \<guillemotleft>real_of_pos t\<guillemotright>)))"
   by (simp add: hyrel2trl_cond hyrel2trel_hEvolves tank_ode_1_evolve tank_ode_2_evolve closure continuous_intros, rel_auto)
+    
+declare rel_frext_skip [frame]
+declare rel_frext_assigns [frame]
+  
+declare arestr_lit [simp]
+declare arestr_false [simp] 
+declare arestr_zero [simp] 
+declare aext_lit [simp]
+  
+lemma st_rel_cond [rpred]:
+  "[P \<triangleleft> b \<triangleright>\<^sub>r Q]\<^sub>S = [P]\<^sub>S \<triangleleft> b \<triangleright>\<^sub>R [Q]\<^sub>S"
+  by (rel_auto)
+ 
+lemma st_subst_assigns_rea [usubst]:
+  "\<sigma> \<dagger>\<^sub>S \<langle>\<rho>\<rangle>\<^sub>r = \<langle>\<rho> \<circ> \<sigma>\<rangle>\<^sub>r"
+  by (rel_auto)
+  
+lemma st_rel_false [rpred]: "[false]\<^sub>S = false"
+  by (rel_auto)
+    
+lemma st_rel_skip [rpred]: 
+  "[II]\<^sub>S = (II\<^sub>r :: ('s, 't::trace) rdes)"
+  by (rel_auto)
+  
+lemma st_subst_rea_skip [usubst]:
+  "\<sigma> \<dagger>\<^sub>S II\<^sub>r = \<langle>\<sigma>\<rangle>\<^sub>r"
+  by (rel_auto)
+
+lemma st_subst_rea_wait [usubst]:
+  "\<sigma> \<dagger>\<^sub>S wait\<^sub>r n = wait\<^sub>r (\<sigma> \<dagger> n) ;; \<langle>\<sigma>\<rangle>\<^sub>r"
+  by (rel_auto)
+    
+lemma lit_plus_appl [lit_simps]: 
+  "\<guillemotleft>op +\<guillemotright>(x)\<^sub>a(y)\<^sub>a = x + y"
+  by (pred_auto)
+
+lemma lit_minus_appl [lit_simps]: 
+  "\<guillemotleft>op -\<guillemotright>(x)\<^sub>a(y)\<^sub>a = x - y"
+  by (pred_auto)
+    
+lemma [usubst]: "ctr \<prec>\<^sub>v tank" 
+  by (simp add: var_name_ord_def)
+        
+lemma [usubst]: "x \<prec>\<^sub>v y \<Longrightarrow> x:a \<prec>\<^sub>v y:b"
+  by (simp add: var_name_ord_def)
+    
+lemma var_name_ord_comp_inner [usubst]: 
+  "a \<prec>\<^sub>v b \<Longrightarrow> x:a \<prec>\<^sub>v x:b"
+  by (simp add: var_name_ord_def)
+
+lemma var_name_ord_pr_var_1 
+  [usubst]: "x \<prec>\<^sub>v y \<Longrightarrow> &x \<prec>\<^sub>v y"
+  by (simp add: var_name_ord_def)
+
+lemma [usubst]: "x \<prec>\<^sub>v y \<Longrightarrow> x \<prec>\<^sub>v &y"
+  by (simp add: var_name_ord_def)
+    
+lemma [usubst]: "level \<prec>\<^sub>v valve"
+  by (simp add: var_name_ord_def)
+
+lemma [usubst]: "ctdown \<prec>\<^sub>v levelSensor"
+  by (simp add: var_name_ord_def)  
+
+lemma [usubst]: "ctdown \<prec>\<^sub>v valveOn"
+  by (simp add: var_name_ord_def)  
+
+lemma [usubst]: "levelSensor \<prec>\<^sub>v valveOn"
+  by (simp add: var_name_ord_def)  
+
+(* The difference between the sensed value of the water level and the actual level is less than 0.1 *)
+    
+lemma wt_prop1:
+  "\<lbrace>true\<rbrace>FMI Init [FMU[ctr, Ctr 0 10], FMU[tank, Tank]] (FixedStep 0.001) Wiring \<lbrace>&tank:level - &ctr:levelSensor <\<^sub>u 0.1\<rbrace>\<^sub>r"
+proof (rule FMI_hoare_rp, simp_all)
+  show "\<lbrace>true\<rbrace> [ctr:[fmiInstantiate (Ctr 0 10)]\<^sup>+ ;; tank:[fmiInstantiate Tank]\<^sup>+]\<^sub>S ;; \<langle>Init\<rangle>\<^sub>r \<lbrace>&tank:level - &ctr:levelSensor <\<^sub>u 0.1\<rbrace>\<^sub>r"
+    by (simp add: Ctr_def Step_VDMRT Tank_def Init_def rpred frame alpha usubst closure, rel_auto)
+  show "\<lbrace>&tank:level - &ctr:levelSensor <\<^sub>u 0.1\<rbrace> 
+          \<langle>Wiring\<rangle>\<^sub>r ;; Step_FMUs [FMU[ctr, Ctr 0 10], FMU[tank, Tank]] (FixedStep (1 / 1000))
+        \<lbrace>&tank:level - &ctr:levelSensor <\<^sub>u 0.1\<rbrace>\<^sub>r"
+    apply (simp add: Wiring_def rpred frame closure usubst Ctr_def Tank_def Step_FMUs_def Step_VDMRT Step_Modelica_FMU HyStep_cond tank_ode_1_evolve tank_ode_2_evolve)
+    apply (simp add: HyStep_hEvolves' closure continuous_intros usubst alpha)
+    apply (uexpr_simp simps:pos_transfer)
+    apply (rel_auto)
+    apply (simp_all add: pos_transfer)
+  done
+qed
+
+method fmi_hoare uses defs =
+  (rule FMI_hoare_rp, 
+   simp_all add:Step_VDMRT Step_Modelica_FMU Step_FMUs_def FixedStep_def HyStep_cond HyStep_hEvolves' closure continuous_intros defs,
+   (simp_all add: frame alpha usubst unrest rpred closure),
+   ((uexpr_simp simps:pos_transfer)[1])?,
+   ((uexpr_simp simps:pos_transfer)[2])?)
+ 
+term cond
+ 
+definition subst_cond :: "'\<alpha> usubst \<Rightarrow> '\<alpha> upred \<Rightarrow> '\<alpha> usubst \<Rightarrow> '\<alpha> usubst" ("(3_ \<triangleleft> _ \<triangleright>\<^sub>s/ _)" [52,0,53] 52) where
+[upred_defs]: "subst_cond \<sigma> b \<rho> = (\<lambda> s. if \<lbrakk>b\<rbrakk>\<^sub>e s then \<sigma>(s) else \<rho>(s))"
+ 
+lemma st_cond_assigns [rpred]:
+  "\<langle>\<sigma>\<rangle>\<^sub>r \<triangleleft> b \<triangleright>\<^sub>R \<langle>\<rho>\<rangle>\<^sub>r = \<langle>\<sigma> \<triangleleft> b \<triangleright>\<^sub>s \<rho>\<rangle>\<^sub>r"
+  by (rel_auto)
+  
+lemma usubst_cond_upd_1 [usubst]:
+  "\<sigma>(x \<mapsto>\<^sub>s u) \<triangleleft> b \<triangleright>\<^sub>s \<rho>(x \<mapsto>\<^sub>s v) = (\<sigma> \<triangleleft> b \<triangleright>\<^sub>s \<rho>)(x \<mapsto>\<^sub>s u \<triangleleft> b \<triangleright> v)"
+  by (rel_auto)
+
+lemma usubst_cond_upd_2 [usubst]:
+  "\<lbrakk> vwb_lens x; x \<sharp> \<rho> \<rbrakk> \<Longrightarrow> \<sigma>(x \<mapsto>\<^sub>s u) \<triangleleft> b \<triangleright>\<^sub>s \<rho> = (\<sigma> \<triangleleft> b \<triangleright>\<^sub>s \<rho>)(x \<mapsto>\<^sub>s u \<triangleleft> b \<triangleright> &x)"
+  by (rel_simp, metis lens_override_def lens_override_idem var_ueval)
+
+lemma usubst_cond_upd_3 [usubst]:
+  "\<lbrakk> vwb_lens x; x \<sharp> \<sigma> \<rbrakk> \<Longrightarrow> \<sigma> \<triangleleft> b \<triangleright>\<^sub>s \<rho>(x \<mapsto>\<^sub>s v) = (\<sigma> \<triangleleft> b \<triangleright>\<^sub>s \<rho>)(x \<mapsto>\<^sub>s &x \<triangleleft> b \<triangleright> v)"
+  by (rel_simp, metis lens_override_def lens_override_idem var_ueval)
+    
+lemma usubst_cond_id [usubst]:
+  "id \<triangleleft> b \<triangleright>\<^sub>s id = id"
+  by (rel_auto)
+    
+lemma cond_true_false [simp]: 
+  "true \<triangleleft> b \<triangleright> false = b"
+  by (rel_auto)
+  
+declare cond_idem [simp]
+  
+term abs
+
+lemma hoare_rp_prune_1 [hoare_safe]:
+  "\<lbrace>p\<rbrace>Q\<lbrace>r\<rbrace>\<^sub>r \<Longrightarrow> \<lbrace>p\<rbrace>false \<triangleleft> b \<triangleright>\<^sub>R Q\<lbrace>r\<rbrace>\<^sub>r"
+  by (rel_auto)
+    
+lemma hoare_rp_wait [hoare_safe]:
+  "\<lbrace>p\<rbrace>wait\<^sub>r n\<lbrace>p\<rbrace>\<^sub>r"
+  by (rel_auto)
+  
+lemma wt_prop2:
+  "\<lbrace>true\<rbrace>
+     FMI Init [FMU[ctr, Ctr 0 10], FMU[tank, Tank]] (FixedStep 0.001) Wiring 
+   \<lbrace>(&tank:level - &ctr:levelSensor =\<^sub>u -0.001) \<triangleleft> &tank:valve \<triangleright> (&tank:level - &ctr:levelSensor =\<^sub>u 0.001)\<rbrace>\<^sub>r"  
+  apply (fmi_hoare defs: Tank_def Ctr_def Init_def Wiring_def tank_ode_1_evolve tank_ode_2_evolve)
+   apply (hoare_auto)
+  apply (uexpr_simp simps:pos_transfer)
+  apply (simp add: rpred closure usubst unrest cond_st_distr)
+  apply (hoare_auto)
+done    
+ 
+lemma wt_prop3:
+  "\<lbrace>true\<rbrace>
+     FMI Init [FMU[ctr, Ctr 0 10], FMU[tank, Tank]] (FixedStep 0.001) Wiring 
+   \<lbrace>(\<not> &tank:valve \<and> &ctr:valveOn) =\<^sub>u (&ctr:levelSensor <\<^sub>u 10 \<and> &tank:level \<ge>\<^sub>u 10) \<and> 
+    (&tank:level - &ctr:levelSensor =\<^sub>u -0.001) \<triangleleft> &tank:valve \<triangleright> (&tank:level - &ctr:levelSensor =\<^sub>u 0.001)\<rbrace>\<^sub>r"  
+  apply (fmi_hoare defs: Tank_def Ctr_def Init_def Wiring_def tank_ode_1_evolve tank_ode_2_evolve)
+   apply (hoare_auto)
+  apply (uexpr_simp simps:pos_transfer)
+  apply (simp add: rpred closure usubst unrest cond_st_distr)
+  apply (hoare_auto)
+  apply (pred_simp)
+ 
+  
+
+    
+proof (rule FMI_hoare_rp, simp_all)
+  show "\<lbrace>true\<rbrace> [ctr:[fmiInstantiate (Ctr 0 10)]\<^sup>+ ;; tank:[fmiInstantiate Tank]\<^sup>+]\<^sub>S ;; \<langle>Init\<rangle>\<^sub>r \<lbrace>&tank:level - &ctr:levelSensor <\<^sub>u 0.1\<rbrace>\<^sub>r"
+    by (simp add: Ctr_def Step_VDMRT Tank_def Init_def rpred frame alpha usubst closure, rel_auto)
+  show "\<lbrace>&tank:level - &ctr:levelSensor <\<^sub>u 0.1\<rbrace> 
+          \<langle>Wiring\<rangle>\<^sub>r ;; Step_FMUs [FMU[ctr, Ctr 0 10], FMU[tank, Tank]] (FixedStep (1 / 1000))
+        \<lbrace>&tank:level - &ctr:levelSensor <\<^sub>u 0.1\<rbrace>\<^sub>r"
+    apply (simp add: Wiring_def rpred frame closure usubst Ctr_def Tank_def Step_FMUs_def Step_VDMRT Step_Modelica_FMU HyStep_cond tank_ode_1_evolve tank_ode_2_evolve)
+    apply (simp add: HyStep_hEvolves' closure continuous_intros usubst alpha)
+    apply (uexpr_simp simps:pos_transfer)
+    apply (rel_auto)
+    apply (simp_all add: pos_transfer)
+  done
+qed
+
+  
+lemma wt_prop2:
+  "\<lbrace>true\<rbrace>FMI Init [FMU[ctr, Ctr 0 10], FMU[tank, Tank]] (FixedStep 0.001) Wiring \<lbrace>&tank:level - &ctr:levelSensor <\<^sub>u 0.1\<rbrace>\<^sub>r"
+  
+  show "\<lbrace>true\<rbrace> 
+           [ctr:[fmiInstantiate (Ctr 0 10)]\<^sup>+ ;; tank:[fmiInstantiate Tank]\<^sup>+]\<^sub>S ;;
+           \<langle>Init\<rangle>\<^sub>r ;; Step_FMUs [FMU[ctr, Ctr 0 10], FMU[tank, Tank]] {1 / 1000} ;; \<langle>Wiring\<rangle>\<^sub>r
+        \<lbrace>\<not> &ctr:valveOn \<Rightarrow> &tank:level \<le>\<^sub>u 11\<rbrace>\<^sub>r"
+     apply (simp add: Ctr_def Step_VDMRT Tank_def Tank_Step Step_FMUs_def)
+     apply (simp add: Step_Modelica_FMU Step_VDMRT HyStep_cond tank_ode_1_evolve tank_ode_2_evolve)
+     apply (simp_all add: HyStep_hEvolves' closure continuous_intros)
+     apply (simp add: frame alpha usubst)
+     apply (simp add: Init_def)
+     apply (simp add: rpred frame Init_def Wiring_def usubst unrest closure alpha)
+     apply (uexpr_simp simps:pos_transfer)
+     apply (simp add: alpha usubst frame rpred closure unrest seqr_assoc)
+     apply (rel_auto)
+  done
+
+    
+lemma "\<lbrace>true\<rbrace>FMI Init [FMU[ctr, Ctr 0 10], FMU[tank, Tank]] (FixedStep 0.001) Wiring \<lbrace>&tank:level \<le>\<^sub>u \<guillemotleft>12\<guillemotright>\<rbrace>\<^sub>r"
+proof (rule FMI_hoare_rp, simp_all add: FixedStep_def, safe, simp_all)
+  show "fmiDoStep FMU[ctr, Ctr 0 10] is RR"
+    by (simp add: Ctr_def fmu_single_def closure)
+  show "fmiDoStep FMU[tank, Tank] is RR"
+    by (simp add: Tank_def fmu_single_def closure)
+  show "\<lbrace>true\<rbrace> 
+           [ctr:[fmiInstantiate (Ctr 0 10)]\<^sup>+ ;; tank:[fmiInstantiate Tank]\<^sup>+]\<^sub>S ;;
+           \<langle>Init\<rangle>\<^sub>r ;; Step_FMUs [FMU[ctr, Ctr 0 10], FMU[tank, Tank]] {1 / 1000} ;; \<langle>Wiring\<rangle>\<^sub>r
+        \<lbrace>&tank:level \<le>\<^sub>u \<guillemotleft>12\<guillemotright>\<rbrace>\<^sub>r"
+     apply (simp add: Ctr_def Step_VDMRT Tank_def Tank_Step Step_FMUs_def)
+     apply (simp add: Step_Modelica_FMU Step_VDMRT HyStep_cond tank_ode_1_evolve tank_ode_2_evolve)
+     apply (simp_all add: HyStep_hEvolves' closure continuous_intros)
+     apply (unliteralise)
+     apply (simp add: frame alpha usubst)
+     apply (simp add: Init_def)
+     apply (simp add: rpred frame Init_def Wiring_def usubst unrest closure alpha)
+     apply (uexpr_simp simps:pos_transfer)
+     apply (simp add: alpha usubst frame rpred closure unrest seqr_assoc)
+    apply (rel_auto)
+  done
+  show "\<lbrace>&tank:level \<le>\<^sub>u \<guillemotleft>12\<guillemotright>\<rbrace> 
+           Step_FMUs [FMU[ctr, Ctr 0 10], FMU[tank, Tank]] {1 / 1000} ;; 
+           \<langle>Wiring\<rangle>\<^sub>r 
+        \<lbrace>&tank:level \<le>\<^sub>u \<guillemotleft>12\<guillemotright>\<rbrace>\<^sub>r"
+   apply (simp add: Tank_def Tank_Step Step_FMUs_def)
+   apply (simp add: Step_Modelica_FMU Step_VDMRT HyStep_cond tank_ode_1_evolve tank_ode_2_evolve)
+   apply (simp_all add: HyStep_hEvolves' closure continuous_intros)
+   apply (uexpr_simp simps:pos_transfer)
+   apply (simp add: rpred frame Init_def Ctr_def Step_FMUs_def Wiring_def Step_VDMRT HyStep_cond usubst unrest closure alpha)
+   apply (uexpr_simp simps:pos_transfer)
+    apply (rel_auto)
+    
+  apply (simp add: Ctr_def fmu_single_def closure)
+    apply (simp add: Tank_def fmu_single_def closure)
+   apply (simp add: Tank_def Tank_Step Step_FMUs_def)
+   apply (simp add: Step_Modelica_FMU Step_VDMRT HyStep_cond tank_ode_1_evolve tank_ode_2_evolve)
+   apply (simp_all add: HyStep_hEvolves' closure continuous_intros)
+
+  apply (simp add: real_of_pos_1 real_of_pos_less_transfer real_of_pos_numeral real_op_pos_div)
+  apply (simp add: Modelica_FMU_def Step_def Tank_Step)
+    
+    apply (subst usubst)
+   apply (subst rpred)
+    apply (simp_all add: closure)
+    apply (rule closure)
+    apply (simp_all add: closure)
+    apply (rule closure)
+      apply (simp_all add: closure)
+        apply (rule closure)
+     apply (simp_all add: closure)
+    apply (rule closure)
+     apply (simp_all add: closure)
+    apply (rule closure) back
+    apply (rule closure) back
+         apply (simp_all add: closure)
+    apply (rule closure) back
+    apply (simp_all)
+
     
 lemma "\<lbrace>true\<rbrace>WaterTank 0 10 10\<lbrace>&tank:level <\<^sub>u 10 \<and> &ctr:levelSensor <\<^sub>u 10\<rbrace>\<^sub>r"
   apply (simp add: conj_comm conj_assoc)
